---
title: Strong Induction Practice \#1
author: Axel Sorenson
date: 1/11/2024
---

**Theorem**\
Consider the sequence: $a_1 = 2$, $a_2 = 4$, $a_n = 5a_{n-1} - 6a_{n-2}$ $\forall
n \geq 3$. Using this sequence, it can be proved that $a_n = 2^n$ for all $n \geq 
1$.

**Base Cases**\
$a_1 = 2$\
$a_2 = 4$\

**Induction Hypothesis**\
Assume that for some integer $k \geq 3$ where $a_k = 5a_{k-1} - 6a_{k-2}$ and
$a_k = 2^k$.

**What To Prove**\
Given the supposition that for some integer $k \geq 3$ where $a_k = 5a_{k-1} - 
6a_{k-2}$ and $a_k = 2^k$, we will show that $a_{k+1} = 2^{k+1}$ is also true.

**Inductive Step**\
\begin{equation}
\tag{1}
a_{k+1} = 5a_{k} - 6a_{k-2} 
\end{equation}

\begin{equation} 
\tag{2}
a_{k+1} = 5(2^k) - 6(2^{k-1})
\end{equation}

\begin{equation}
\tag{3}
a_{k+1} = 5(2^k) - 6(2^k \cdot \frac{1}{2})
\end{equation}

\begin{equation}
\tag{4}
a_{k+1} = 5(2^k) - 3(2^k)
\end{equation}

\begin{equation}
\tag{5}
a_{k+1} = 2(2^k)
\end{equation}

\begin{equation}
\tag{6}
a_{k+1} = 2^{k+1}
\end{equation}

**Conclusion**\
Therefore, for all $k \geq 1$ given the sequence $a_1 = 2$ and $a_2 = 4$ where 
$a_k = 5a_{k-1} - 6a_{k-2}$ $\forall n \geq 3$, $a_k = 2^k$.
